wip: stuck on defining recursor for `iTree` quotient

IterTree/Basic.lean
@@ -145,19 +145,32 @@ only with its interface, which is what we do theorems againsts.
 -/
 
 
+@[grind cases]
 inductive Obs (E : Type q → Type r) (R : Type v) (K : Type k) where
 | ret : R → Obs E R K
 | tau : K → Obs E R K
 | vis {A : Type q} : E A → (A → K) → Obs E R K
 
+def Obs.mapState (f : α → β) : Obs E R α → Obs E R β 
+| .ret v => .ret v
+| .tau st => .tau <| f st
+| .vis ev k => .vis ev (fun x => f (k x))
+
+def Obs.bindVal (f : α → Obs E β K) : Obs E α K → Obs E β K
+| .ret v => f v
+| .tau st => .tau st
+| .vis ev k => .vis ev k
+
+
 /- class IsITreeImpl (State : Type s) (E : Type q → Type r) (R : Type v) where -/
 /-     step : State → Obs E R State -/
 
 structure iTree (E : Type q → Type r) (R : Type v) where
-  {State : Type s}
+  {State : Type s} -- TODO: Maybe rename to MetaState
   curr : State
   /- [stepImpl : IsITreeImpl State E R] -/
-  step : State → Obs E R (iTree E R)
+  step : State → Obs E R State
+
   -- Why not have it give observations on just `State`?
   -- I think it's not possible, because we must be able to change
   -- the state type at some point in the execution.
@@ -167,18 +180,23 @@ structure iTree (E : Type q → Type r) (R : Type v) where
   -- You can't, you'd need to reference back to the think you're
   -- defining, but at that point it's no longer a fixpoint!
 
-instance : Inhabited (iTree E R) where
-  default := {
-    State := Unit
-    curr := ()
-    step := fun _ => .tau 
-  }
-
-variable {E : Type q → Type r}{R : Type v}
-  
-
-def iTree.unfold (it : iTree E R) : Obs E R (iTree E R) := it.step it.curr 
-
+  -- In short, it can't be State → Obs E R (iTree E R) because
+  -- then one can't really give an infinitely looping computation
+  -- It also can't be `State → Obs E R State` because one should
+  -- be able to encode that the state changes from one computation
+  -- to another. Or can't it?
+  -- 
+  -- The issue with doing this encoding is that one must fix the 
+  -- type of the state of the final computation, but it's not
+  -- trivial to define. For instance, one would like to say that
+  -- when doing a `bind` with `f`, the state will originally be 
+  -- that of the interaction tree being executed, until it gives
+  -- a value `a`, at which point one switches to the state of the 
+  -- `iTree` resulting from applying `f` to `a`. However, this 
+  -- cannot be expressed directly as a type.
+  -- One could, however, express this as an invariant of the 
+  -- structure, which leads us back to the `IsPlausibleStep` of 
+  -- `Std.Iter`.
 /-
 
 An alternate representation of this interface would be to have `curr : State` be the implementation of
@@ -188,37 +206,791 @@ an `iTree E R`, and assign to each `State` type a particular `step` function.
 
 namespace iTree
 
-variable {E : Type q → Type r}
+variable {E : Type q → Type r} {R : Type v}
 
-/- instance : Inhabited ({E : Type q → Type r} → {α : Type u_1} → {β : Type u_2} → (α → iTree E β) → iTree E α → iTree E β) where -/
-/-   default f it := { -/
-    
-/-   } -/
+/-- The looping computation -/
+def loop.{s} : iTree E R where
+  State := PUnit.{s+1}
+  curr := .unit
+  step _ := .tau .unit
+
+set_option pp.universes true in #print loop
+
+instance : Inhabited (iTree E R) := ⟨loop⟩
+  
+def unfold (it : iTree E R) : Obs E R (iTree E R) := 
+  match it.step it.curr with 
+  | .ret v => .ret v
+  | .tau next => .tau {it with curr := next}
+  | .vis ev k => .vis ev (fun x => {it with curr := (k x)})
+
+theorem unfold_cases (it : iTree E R) :
+    (∃ v, it.unfold = .ret v) ∨
+    (∃ (α : Type _) (ev : E α) (k : α → iTree E R), it.unfold = .vis ev k) ∨ 
+    (∃ it', it.unfold = .tau it') := 
+  match it.unfold with 
+  | .ret v => .inl ⟨v, rfl⟩
+  | .vis (A := α) ev k => .inr <| .inl ⟨α, ev, k, rfl⟩
+  | .tau next => .inr <| .inr ⟨next, rfl⟩
+/- grind_pattern unfold_cases => it.unfold -/
+-- NOTE: It might be enough with [grind cases] on `Obs`.
+
+-- Maybe this can be defined later, once we have equality over unfoldings.
+/- def recUnfold {motive : iTree E R → Prop} -/
+/-   (onRet : (v : R) → motive (.ret v)) -/
+/-   (onTau : (it iTree E R → -/ 
+
+def ret (r : R) : iTree E R where
+  curr : Unit  := ()
+  step _ := .ret r
+
+set_option pp.universes true in #print ret
+
+def vis {α} (ev : E α) (k : α → iTree E R) : iTree E R where
+  curr : Unit ⊕ (a : α) × (k a ).State := .inl ()
+  step 
+  | .inl () => .vis ev (fun a => .inr <| ⟨a, (k a).curr⟩)
+  | .inr ⟨a, s⟩ => (k a).step s |>.mapState (.inr ⟨a, ·⟩)
+
+def tau (it : iTree E R) : iTree E R where
+  -- We basically generate an artificial prior element in the state.
+  curr : Unit ⊕ it.State  := .inl ()
+  step
+  | .inl () => .tau <| .inr <| it.curr
+  | .inr s => it.step s |>.mapState (.inr)
+
+end iTree
+
+def Obs.toITree : Obs E R (iTree E R) → iTree E R 
+| .tau it => iTree.tau it
+| .vis ev k => iTree.vis ev k
+| .ret v => iTree.ret v
+  
+
+namespace iTree
+
 
 /--
   After the computation of the interaction tree `it`, we simply continue with the
   computation given by `f`. We encode the information of the continuation in the 
   closure, to dodge problems with termination.
 -/
-partial
-def bindLeft {α β} (f : α → iTree E β)(it : iTree E α) : iTree E β :=
-  {
-    State := it.State
-    curr := it.curr
-    step st := match it.step st with
-      | .ret r => .tau (f r)
-      | .tau it => .tau (it.bindLeft f)
-      | .vis ev k => 
-        .vis ev (fun a => (k a).bindLeft f)
-  }
+def bindLeft {α β} (f : α → iTree E β)(it : iTree E α) : iTree E β where
+    curr : it.State ⊕ (a : α) × (f a).State := .inl it.curr
+    step st := 
+      match st with 
+      | .inl curr =>
+        it.step curr 
+        |>.mapState .inl 
+        |>.bindVal (fun a => .tau <| .inr ⟨a, (f a).curr⟩)
+      | .inr ⟨a, st⟩ =>
+        (f a).step st 
+        |>.mapState (.inr ⟨a, ·⟩)
 
-/- instance : Bind (iTree E) := ⟨(·.bindLeft ·)⟩ -/
-/- instance : Pure (iTree E) := ⟨.ret⟩ -/
-/- instance : Monad (iTree E) where -/
-/- instance  : LawfulMonad (iTree E) := .mk' -/
-/-    (id_map     := by intros α it; simp only [Functor.map, bind, pure, Function.comp_id]; induction it <;> simp [bindLeft, *] ) -/
-/-    (pure_bind  := by intros α β it f; simp only [bind, bindLeft]) -/
-/-    (bind_assoc := by intros α β γ it f g; simp only [bind]; induction it <;> simp [bindLeft, *]) -/
+instance : Bind (iTree E) := ⟨(·.bindLeft ·)⟩
+instance : Pure (iTree E) := ⟨ret⟩
+instance : Monad (iTree E) where
+
+/- def iter {I} (step : I → iTree E (I ⊕ R)) (init : I) : iTree E R := -/
+/-   (step init).bindLeft fun -/
+/-   | .inl updated => .tau (iter step updated) -/
+/-   | .inr res => .ret res -/
+def iter {I} (f : I → iTree E (I ⊕ R)) (init : I) : iTree E R where
+  curr : (i : I) × (f i).State := ⟨init, f init |>.curr⟩
+  step
+  | ⟨i, st⟩ =>
+    (f i).step st
+    |>.mapState (⟨i, ·⟩)
+    |>.bindVal fun
+    | .inl i' => .tau <| ⟨i', (f i').curr⟩
+    | .inr res => .ret res
+
+section EqualitiesOverITrees
+
+/-
+
+There are actually many notions of equality that can be given to iTrees.
+
+There's strict equality, which is not very useful. In particular, you have
+to care about the internal state of your iTree.
+
+Then there is an "extensional" equality, or "observational" equality, which
+cares only for the observable behaviour of iTrees. In particular, it does
+away with the details of the internal state, and only cares for the `Obs`
+produced by the `step` function. 
+
+However, this is not the best notion of equality either. We also have
+equivalences between iTrees which are equivalent in their observations if
+we're allowed to skip a finite amount of `tau` steps from either `iTree`.
+This notion is called "equivalence up to tau", and captures more faithfully
+the concept of what a "computation" is.
+-/
+
+namespace WrongEq
+
+/-- 
+  This is the wrong notion of equality!
+
+  It allows one to identify `fun _ => .ret 0` with `.skip`!
+-/
+def eq {α} (it₁ it₂ : iTree E α) : Prop := 
+  match it₁.unfold, it₂.unfold with
+  | .ret v₁, .ret v₂ => v₁ = v₂
+  | @Obs.vis _ _ _ A₁ ev₁ k₁, @Obs.vis _ _ _ A₂ ev₂ k₂ =>
+    ∃ (h : A₁ = A₂), ev₁ ≍ ev₂ ∧ ∀ a, eq (k₁ a) (k₂ (h.mp a))
+  | .tau it₁, _
+  | _, .tau it₂ => eq it₁ it₂
+  | _, _ => False
+coinductive_fixpoint monotonicity fun f f' himp => by
+  intro it₁ it₂ 
+  match h : it₁.unfold with
+  | .ret v₁ =>
+    simp only [h]
+    match it₂.unfold with
+    | .ret v₁ =>
+      simp only
+      intro h; exact h
+    | @Obs.vis _ _ _ A₁ ev₁ k₁ =>
+      simp only
+      intro h; exact h
+    | .tau it₁ =>
+      simp only
+      intro h
+      apply himp
+      exact h
+  | @Obs.vis _ _ _ A₁ ev₁ k₁ =>
+    simp only [h]
+    match h : it₂.unfold with
+    | .ret v₁ =>
+      simp only
+      intro h; exact h
+    | @Obs.vis _ _ _ A₁ ev₁ k₁ =>
+      simp only
+      rintro ⟨rfl, rfl, hk⟩
+      refine ⟨rfl, ?_⟩
+      refine ⟨.rfl, ?_⟩
+      intro a 
+      specialize hk a
+      apply himp
+      exact hk
+    | .tau it₁ =>
+      simp only
+      intro h
+      apply himp
+      exact h
+  | .tau it₁ =>
+    simp only [h]
+    match it₂.unfold with
+    | .ret v₁ =>
+      intro h
+      apply himp
+      exact h
+    | @Obs.vis _ _ _ A₁ ev₁ k₁ =>
+      intro h
+      apply himp
+      exact h
+    | .tau it₁ =>
+      intro h
+      apply himp
+      exact h
+
+end WrongEq
+
+/-
+
+To define the right notion, we have to define what is a weak bisimulation.
+
+-/
+
+namespace FirstTry
+
+inductive wb (r : iTree E V → iTree E V → Prop) : iTree E V → iTree E V → Prop where
+| ret  : ∀ v : V,                  wb r (.ret v) (.ret v)
+| sync : ∀ it₁ it₂,    r it₁ it₂ → wb r (.tau it₁) (.tau it₂)
+| tauL : ∀ it₁ it₂, wb r it₁ it₂ → wb r (.tau it₁) it₂
+| tauR : ∀ it₁ it₂, wb r it₁ it₂ → wb r (.tau it₁) it₂
+| vis  : ∀ ev₁ k₁ ev₂ k₂, ev₁ = ev₂ → (∀ a, r (k₁ a) (k₂ a)) → wb r (.vis ev₁ k₁) (.vis ev₂ k₂)
+-- Does this work? We can't really pattern match on `it`.
+
+-- Maybe we can fix it with this?
+public def wb' (r : iTree E V → iTree E V → Prop) (it₁ it₂ : iTree E V) : Prop :=
+   wb r it₁.unfold.toITree it₂.unfold.toITree
+
+def bisimulation : iTree E V → iTree E V → Prop := wb bisimulation
+coinductive_fixpoint monotonicity fun r r' himp => by
+  intro it₁ it₂ H
+  induction H with 
+  | ret v =>  constructor
+  | sync it₁ it₂ R =>
+    constructor; apply himp; assumption
+  | vis ev k => 
+    constructor
+    · assumption
+    · intros; apply himp; grind only
+  | tauL it₁ it₂ _ IH =>
+    constructor; assumption
+  | tauR it₁ it₂ _ IH =>
+    constructor; assumption
+
+/-
+
+However, this definition doesn't work because we can't identify every possible
+iTree in terms of construction of `.tau`, `.vis` and `.ret`. We have no destructor
+for `iTree`!
+
+-/
+
+end FirstTry
+
+namespace SecondTry
+
+public inductive wb (r : iTree E V → iTree E V → Prop) : iTree E V → iTree E V → Prop where
+| ret {it₁ it₂}  : ∀ v : V, 
+    it₁.unfold = .ret v → it₂.unfold = .ret v →
+    wb r it₁ it₂
+| vis  {it₁ it₂} : ∀ ev₁ k₁ ev₂ k₂,
+    it₁.unfold = .vis ev₁ k₁ → it₂.unfold = .vis ev₂ k₂ → -- Maybe even these equalities are a bit much…
+    ev₁ = ev₂ → (∀ a, r (k₁ a) (k₂ a)) →
+    wb r it₁ it₂
+| sync {it₁ it₂} : ∀ it₁' it₂',
+    it₁.unfold = .tau it₁' → it₂.unfold = .tau it₂' →
+    r it₁' it₂' →
+    wb r it₁ it₂
+| tauL {it₁ it₂} : ∀ it₁',
+    it₁.unfold = .tau it₁' →
+    wb r it₁' it₂ → 
+    wb r it₁ it₂
+| tauR {it₁ it₂} : ∀ it₂', 
+    it₂.unfold = .tau it₂' →
+    wb r it₁ it₂ → wb r it₁ it₂
+
+def eq : iTree E V → iTree E V → Prop := wb eq
+coinductive_fixpoint monotonicity fun r r' himp => by
+  intro it₁ it₂ H
+  induction H with 
+  | ret v h₁ h₂ => 
+    apply wb.ret v h₁ h₂
+  | sync it₁ it₂ h₁ h₂ R =>
+    apply wb.sync it₁ it₂ h₁ h₂
+    apply himp; assumption
+  | vis ev₁ k₁ ev₂ k₂ h₁ h₂ hev IH => 
+    apply wb.vis ev₁ k₁ ev₂ k₂ h₁ h₂ hev
+    intros; apply himp; grind
+  | tauL it₁' h₁ _ IH =>
+    apply wb.tauL it₁' h₁ IH
+  | tauR it₂' h₂ _ IH =>
+    apply wb.tauR it₂' h₂ IH
+-- TODO: Is this the correct notion of equality?
+-- TODO: Is this equivalent to `FirstTry.bisimulation`?
+--       Or what's equivalent, is `FirstTry.wb'` equivalent to `wb` here?
+
+end SecondTry
+
+namespace ThirdTry
+
+/-
+
+We define a weaker version of equality, observational
+
+-/
+
+-- TODO: Maybe it'd be cool to define it as a mutually recursive relation.
+-- where we have relatiosn between Obs E R (iTree E R) and iTree E R defined
+-- in terms of one another.
+-- Might be useful for grind lemmas.
+
+mutual 
+  variable {R : Type _}{E : Type _ → Type _}
+
+  abbrev Rel (r : R → R → Prop) (it₁ it₂ : iTree E R)  : Prop := ObsRel r it₁.unfold it₂.unfold
+  coinductive_fixpoint monotonicity by
+    rintro Rel Rel' ⟨_, Obsimp⟩ it₁ it₂ H
+    apply Obsimp
+    assumption
+
+  def ObsRel (r : R → R → Prop) : Obs E R (iTree E R) → Obs E R (iTree E R) → Prop
+  | .ret v₁, .ret v₂ => 
+      r v₁ v₂
+  | .vis (A := A₁) ev₁ k₁, .vis (A := A₂) ev₂ k₂ =>
+      ∃ (h : A₁ = A₂), ev₁ = h ▸ ev₂ ∧ ∀ s₁, 
+        Rel r (k₁ s₁) (k₂ (h ▸ s₁))
+  | .tau it₁', .tau it₂' =>
+      Rel r it₁' it₂'
+  | _, _ => False
+  coinductive_fixpoint monotonicity by
+    rintro ⟨Rel, Obs⟩ ⟨Rel', Obs'⟩ ⟨Rimp, _⟩ obs₁ obs₂ H
+    match h₁ : obs₁ with 
+    | .ret v₁ => 
+        cases h₂ : obs₂ <;> grind
+    | .vis (A := A₁) ev₁ k₁ => 
+        match obs₂ with 
+        | .ret v₂ => grind
+        | .tau it₂ => grind
+        | .vis (A := A₂) ev₂ k₂ => 
+          obtain ⟨h, rfl, ext⟩ := H
+          simp only [Lean.Order.PartialOrder.rel, true_and, h, exists_true_left] at *
+          intros; apply Rimp; apply ext
+    | .tau it₁ => 
+        match  obs₂ with 
+        | .ret v₂ => grind
+        | .vis (A := A₂) ev₂ k₂ => grind
+        | .tau it₂ =>
+          apply Rimp
+          assumption
+
+end
+
+
+abbrev ObsRel.func (s : iTree E R → iTree E R → Prop) (r : R → R → Prop) : Obs E R (iTree E R) → Obs E R (iTree E R) → Prop
+| .ret v₁, .ret v₂ => 
+    r v₁ v₂
+| .vis (A := A₁) ev₁ k₁, .vis (A := A₂) ev₂ k₂ =>
+    ∃ (h : A₁ = A₂), ev₁ = h ▸ ev₂ ∧ ∀ s₁, 
+      s (k₁ s₁) (k₂ (h ▸ s₁))
+| .tau it₁', .tau it₂' =>
+    s it₁' it₂'
+| _, _ => False
+
+/- def ObsRel (r : R → R → Prop)(it₁ it₂ : iTree E R) : Prop := -/ 
+/-   match it₁.unfold, it₂.unfold with -/ 
+/-   | .ret v₁, .ret v₂ => -/ 
+/-       r v₁ v₂ -/
+/-   | .vis (A := A₁) ev₁ k₁, .vis (A := A₂) ev₂ k₂ => -/
+/-       ∃ (h : A₁ = A₂), ev₁ = h ▸ ev₂ ∧ ∀ s₁, -/ 
+/-         ObsRel r (k₁ s₁) (k₂ (h ▸ s₁)) -/
+/-   | .tau it₁', .tau it₂' => -/
+/-       ObsRel r it₁' it₂' -/
+/-   | _, _ => False -/
+/- coinductive_fixpoint monotonicity fun ObsRel ObsRel' Himp it₁ it₂ H => by -/
+/-   dsimp at H ⊢ -/ 
+/-   match h₁ :  it₁.unfold with -/ 
+/-   | .ret v₁ => -/ 
+/-       simp [h₁] at H ⊢ -/ 
+/-       cases h₂ : it₂.unfold <;> grind -/
+/-   | .vis (A := A₁) ev₁ k₁ => -/ 
+/-       simp [h₁] at H ⊢ -/ 
+/-       match h₂ : it₂.unfold with -/ 
+/-       | .ret v₂ => grind -/
+/-       | .tau it₂ => grind -/
+/-       | .vis (A := A₂) ev₂ k₂ => -/ 
+/-         simp [h₂] at H ⊢ -/ 
+/-         obtain ⟨h, rfl, ext⟩ := H -/
+/-         subst h -/
+/-         simp -/ 
+/-         intros -/
+/-         apply Himp -/
+/-         apply ext -/
+/-   | .tau it₁ => -/ 
+/-       simp [h₁] at H ⊢ -/ 
+/-       match h₂ : it₂.unfold with -/ 
+/-       | .ret v₂ => grind -/
+/-       | .vis (A := A₂) ev₂ k₂ => grind -/
+/-       | .tau it₂ => -/
+/-         simp [h₂] at H ⊢ -/ 
+/-         apply Himp -/
+/-         assumption -/
+
+abbrev ObsEq{E R} (it₁ it₂ : iTree E R) := Rel (· = ·) it₁ it₂
+
+abbrev ObsEq.func s (obs₁ obs₂ : Obs E R (iTree E R)) := ObsRel.func s (·=·) obs₁ obs₂
+
+instance {E : Type _ → Type _} : HasEquiv (iTree E R) where
+  Equiv := ObsEq
+
+/- @[grind →] -/
+/- theorem ObsEq.cases (it₁ it₂ : iTree E R) : -/
+/-     it₁ ≈ it₂ → -/
+/-     (∃ v₁, it₁.unfold = .ret v₁) ∧ (∃ v₂, it₂.unfold = .ret v₂) ∨ -/
+/-     (∃ (A₁ : Type) (ev₁ : E A₁) (k₁ : A₁ → iTree E R), it₁.unfold = .vis ev₁ k₁) ∧ -/ 
+/-     (∃ (A₂ : Type) (ev₂ : E A₂) (k₂ : A₂ → iTree E R), it₂.unfold = .vis ev₂ k₂) ∨ -/
+/-     (∃ it₁', it₁.unfold = .tau it₁') ∧ (∃ it₂', it₂.unfold = .tau it₂') := fun h => -/
+/-   match h₁ : it₁.unfold, h₂ : it₂.unfold with -/ 
+/-   | .ret v₁, .ret v₂ => by grind -/
+/-   | .vis (A := A₁) ev₁ k₁, .vis (A := A₂) ev₂ k₂ => by grind -/
+/-   | .tau it₁', .tau it₂' => by grind -/
+/-   | .ret .., .tau .. -/
+/-   | .ret .., .vis .. -/
+/-   | .vis .., .ret .. -/
+/-   | .vis .., .tau .. -/
+/-   | .tau .., .vis .. -/
+/-   | .tau .., .ret .. => by simp only [h₁, h₂, ObsRel] at h -/
+
+@[grind →]
+theorem ObsEq.obsEq_unfold_eq_ret {it₁ it₂ : iTree E R} :
+    it₁.unfold = .ret v₁ → 
+    it₁ ≈ it₂ →
+    ∃ v₂, it₂.unfold = .ret v₂ := fun h₁ h => by
+  unfold Rel at h
+  cases h₂ : it₂.unfold <;> simp [h₁, h₂, ObsRel] at h
+  case ret v₂ => exists v₂
+
+@[grind →]
+theorem ObsEq.obsEq_unfold_eq_vis {it₁ it₂ : iTree E R} {ev₁ : E A₁} {k₁} :
+    it₁.unfold = .vis ev₁ k₁ → 
+    it₁ ≈ it₂ →
+    ∃ (A₂ : Type _) (ev₂ : E A₂) (k₂ : A₂ → iTree E R), it₂.unfold = .vis ev₂ k₂ := fun h₁ h => by
+  unfold Rel at h
+  cases h₂ : it₂.unfold <;> simp [h₁, h₂, ObsRel] at h
+  case vis A₂ ev₂ k₂ => exists A₂, ev₂, k₂
+
+@[grind →]
+theorem ObsEq.obsEq_unfold_eq_tau {it₁ it₂ it₁' : iTree E R} :
+    it₁.unfold = .tau it₁' → 
+    it₁ ≈ it₂ →
+    ∃ it₂', it₂.unfold = .tau it₂' := fun h₁ h => by
+  unfold Rel at h
+  cases h₂ : it₂.unfold <;> simp [h₁, h₂, ObsRel] at h
+  case tau it₂ => exists it₂
+
+theorem ObsEq.unfold_eq_ret {it₁ it₂ : iTree E R} {v₁ : R} {v₂ : R} :
+    it₁.unfold = .ret v₁ → 
+    it₂.unfold = .ret v₂ →
+    it₁ ≈ it₂ →
+    v₁ = v₂ := fun h₁ h₂ h => by
+  unfold Rel at h
+  simpa [h₁, h₂, ObsRel] using h
+
+theorem ObsEq.unfold_eq_vis {it₁ it₂ : iTree E R} {ev₁ : E A₁} {ev₂ : E A₂} {k₁ k₂} :
+    it₁.unfold = .vis ev₁ k₁ → 
+    it₂.unfold = .vis ev₂ k₂ →
+    it₁ ≈ it₂ →
+    ∃ (h : A₁ = A₂), ev₁ = h ▸ ev₂ ∧ ∀ s₁, 
+      (k₁ s₁) ≈ (k₂ (h ▸ s₁)) := fun h₁ h₂ h => by
+  unfold Rel at h
+  simpa [h₁, h₂, ObsRel] using h
+
+theorem ObsEq.unfold_eq_tau {it₁ it₂ it₁' : iTree E R} :
+    it₁.unfold = .tau it₁' → 
+    it₂.unfold = .tau it₂' →
+    it₁ ≈ it₂ →
+    it₁' ≈ it₂' := fun h₁ h₂ h => by
+  unfold Rel at h
+  simpa [h₁, h₂, ObsRel] using h
+
+@[grind =, grind =_]
+theorem ObsRel.iff_rel {it₁ it₂ : iTree E R} :
+    it₁ ≈ it₂ ↔ ObsRel (·=·) it₁.unfold it₂.unfold := by
+  unfold Rel
+  exact ⟨id, id⟩
+
+    /- /1- set_option pp.all true in -1/ -/
+def ObsEq.coinductWith
+  (pred : iTree E R → iTree E R → Prop) 
+  {it₁ it₂ : iTree E R} 
+  (baseCase : pred it₁ it₂)
+  (progress :
+    ∀ (it₁ it₂ : iTree E R),
+      pred it₁ it₂ → func pred it₁.unfold it₂.unfold) :
+    ObsEq it₁ it₂ := by
+  apply Rel.coinduct (·=·) (pred_1 := pred) (pred_2 := ObsEq.func pred) _ _ _ _ baseCase
+  all_goals grind only
+
+theorem ObsEq.refl (it : iTree E R) : it ≈ it := by 
+  apply ObsEq.coinductWith (·=·) rfl
+  grind only
+ 
+theorem ObsEq.symm (it₁ it₂ : iTree E R) : it₁ ≈ it₂ → it₂ ≈ it₁ := by 
+  intro h
+  apply ObsEq.coinductWith (pred := fun x y => y ≈ x) h 
+  intros it₁ it₂ hyp
+  match h₁ : it₁.unfold, h₂ : it₂.unfold with 
+  | Obs.ret _, Obs.ret _ => 
+    grind [ObsEq.unfold_eq_ret]
+  | Obs.vis (A := A₁) ev₁ k₁, Obs.vis (A := A₂) ev₂ k₂ =>
+    grind [ObsEq.unfold_eq_vis]
+  | Obs.tau it₁', Obs.tau it₂' =>
+    grind [ObsEq.unfold_eq_tau]
+  | .ret .., .tau ..
+  | .ret .., .vis ..
+  | .vis .., .ret ..
+  | .vis .., .tau ..
+  | .tau .., .vis ..
+  | .tau .., .ret .. => 
+    unfold Rel at hyp
+    simp [h₁, h₂,  ObsRel] at hyp
+
+theorem ObsEq.trans (it₁ it₂ it₃ : iTree E R) : it₁ ≈ it₂ → it₂ ≈ it₃ → it₁ ≈ it₃ := by 
+  intro it12 it23
+  apply ObsEq.coinductWith (pred := fun x z => ∃ y, x ≈ y ∧ y ≈ z) ⟨it₂, it12, it23⟩
+  rintro it₁ it₃ ⟨it₂, it12, it23⟩
+  match h₁ : it₁.unfold, h₃ : it₃.unfold with 
+  | Obs.ret _, Obs.ret _ => 
+    grind [ObsEq.unfold_eq_ret]
+  | Obs.vis (A := A₁) ev₁ k₁, Obs.vis (A := A₃) ev₃ k₃ =>
+    grind [ObsEq.unfold_eq_vis]
+  | Obs.tau it₁', Obs.tau it₃' =>
+    unfold func ObsRel.func
+    have ⟨it₂', h₂⟩ := ObsEq.obsEq_unfold_eq_tau h₁ it12
+    have it'12 := ObsEq.unfold_eq_tau h₁ h₂ it12
+    have it'23 := ObsEq.unfold_eq_tau h₂ h₃ it23
+    exists it₂'
+  | .ret .., .tau ..
+  | .ret .., .vis ..
+  | .vis .., .ret ..
+  | .vis .., .tau ..
+  | .tau .., .vis ..
+  | .tau .., .ret .. => 
+    have oit12 := ObsRel.iff_rel.1 it12
+    have oit23 := ObsRel.iff_rel.1 it23
+    grind
+
+instance : Std.Refl (@ObsEq E R) where refl := ObsEq.refl
+instance : Std.Symm (@ObsEq E R) where symm := ObsEq.symm
+instance : Trans (@ObsEq E R) (@ObsEq E R) (@ObsEq E R) where trans := ObsEq.trans _ _ _
+
+def ObsEq.step_tau_obsEq_self (it : iTree E R) (s : it.State) c : 
+    { {it with curr := c}.tau with curr := .inr s } ≈ {it with curr := s} := by
+  apply ObsEq.coinductWith (fun 
+    (iTree.mk (State := State₁) curr₁ step₁) 
+    (iTree.mk (State := State₂) curr₂ step₂) =>
+    ∃ (H : State₁ = (Unit ⊕ State₂)),
+    curr₁ = H.mpr (Sum.inr curr₂) ∧
+    ∀ (s : State₂), 
+    step₁ (H ▸ (.inr s)) = H.symm ▸ (step₂ s).mapState .inr
+  )
+  case baseCase => 
+    simp [tau, Obs.mapState]
+  case progress =>
+    unfold func ObsRel.func unfold
+    rintro ⟨c₁, s₁⟩ ⟨c₂, s₂⟩ ⟨rfl, HC, Hs⟩
+    cases _ : s₁ c₁ <;>
+    cases _ : s₂ c₂ <;>
+    simp [*, Obs.mapState]
+
+def ObsEq.step_vis_obsEq_self {E R A} (it : iTree E R) (ev : E A) (kS : A → it.State) (a : A) :
+    { curr := kS a, step := it.step : iTree E R} ≈
+    { curr : Unit ⊕ (_ : A) × it.State := Sum.inr ⟨a, kS a⟩,
+        step := fun x =>
+          match x with
+          | Sum.inl PUnit.unit => Obs.vis ev fun a => Sum.inr ⟨a, kS a⟩
+          | Sum.inr ⟨a, s⟩ => Obs.mapState (fun x => Sum.inr ⟨a, x⟩) (it.step s) } := by
+  apply ObsEq.coinductWith (fun 
+    (iTree.mk (State := State₁) curr₁ step₁) 
+    (iTree.mk (State := State₂) curr₂ step₂) =>
+    ∃ (H : State₂ = (Unit ⊕ (_ : A) × State₁)),
+    curr₂ = H.mpr (Sum.inr ⟨a, curr₁⟩) ∧
+    ∀ (s : State₁), 
+    step₂ (H ▸ (.inr ⟨a, s⟩)) = H.symm ▸ (step₁ s).mapState (.inr ⟨a, ·⟩)
+  )
+  case baseCase => 
+    simp [Obs.mapState]
+  case progress =>
+    rintro ⟨c₁, s₁⟩ ⟨c₂, s₂⟩ ⟨rfl, HC, Hs⟩
+    unfold ObsEq.func ObsRel.func unfold
+    cases _ : s₁ c₁ <;>
+    cases _ : s₂ c₂ <;>
+    simp [*, Obs.mapState]
+
+/- def ObsEq.step_vis_obsEq_self {E : Type _ → Type _}(ev : E A) (k : A → S) (a : A) (s : S) c : -/ 
+    /- { iTree.vis ev (fun a => ⟨c, k a⟩) with curr := .inr ⟨a, s⟩ } ≈ {it with curr := s} := by -/
+  /- apply ObsEq.coinductWith (fun -/ 
+  /-   (iTree.mk (State := State₁) curr₁ step₁) -/ 
+  /-   (iTree.mk (State := State₂) curr₂ step₂) => -/
+  /-   ∃ (H : State₁ = (Unit ⊕ State₂)), -/
+  /-   curr₁ = H.mpr (Sum.inr curr₂) ∧ -/
+  /-   ∀ (s : State₂), -/ 
+  /-   step₁ (H ▸ (.inr s)) = H.symm ▸ (step₂ s).mapState .inr -/
+  /- ) -/
+  /- case baseCase => -/ 
+  /-   simp [tau, Obs.mapState] -/
+  /- case progress => -/
+  /-   unfold func ObsRel.func unfold -/
+  /-   rintro ⟨c₁, s₁⟩ ⟨c₂, s₂⟩ ⟨rfl, HC, Hs⟩ -/
+  /-   cases _ : s₁ c₁ <;> -/
+  /-   cases _ : s₂ c₂ <;> -/
+  /-   simp [*, Obs.mapState] -/
+
+theorem ObsEq.tau_congr {it₁ it₂ : iTree E R} : it₁ ≈ it₂ → (iTree.tau it₁) ≈ (iTree.tau it₂) := by
+  intro h
+  unfold Rel
+  simp [unfold, tau, ObsRel]
+  change ({ it₁.tau with curr := .inr it₁.curr } ≈ { it₂.tau with curr := .inr it₂.curr })
+  calc { it₁.tau with curr := .inr it₁.curr }
+    _ ≈ (it₁ : iTree E R) := step_tau_obsEq_self ..
+    _ ≈ it₂ := h
+    _ ≈ { it₂.tau with curr := .inr it₂.curr } := (step_tau_obsEq_self ..).symm
+
+theorem ObsEq.obsEq_ret_of_unfold_ret {it : iTree E R} {v : R} : it.unfold = .ret v → it ≈ .ret v := by
+  simp [unfold]
+  cases h : it.step it.curr <;> simp
+  rintro rfl
+  unfold Rel ObsRel unfold
+  simp [h, ret]
+
+theorem ObsEq.obsEq_tau_of_unfold_tau {it it': iTree E R} : it.unfold = .tau it' → it ≈ .tau it' := by
+  simp [unfold]
+  cases h : it.step it.curr <;> simp
+  case tau st =>
+    rintro rfl
+    unfold Rel ObsRel unfold
+    have := step_tau_obsEq_self it st st |>.symm
+    simpa [tau, h]
+
+set_option pp.universes true in
+theorem ObsEq.obsEq_vis_of_unfold_vis {it : iTree E R}{ev : E A} {k}: it.unfold = .vis ev k → it ≈ .vis ev k := by
+  simp [unfold]
+  cases h : it.step it.curr <;> simp
+  case vis A ev kS =>
+    rintro rfl rfl rfl
+    unfold Rel ObsRel unfold
+    simp [vis, h]
+    intros a
+    /- have := ObsEq.step_vis_obsEq_self it ev kS a -/
+    /- dsimp [HasEquiv.Equiv, instHasEquiv, ObsEq] at this -/
+    /- assumption -/
+    -- TODO: Idk why I can't conclude with the previous, so I just copy-paste the proof
+    -- of `ObsEq.step_vis_obsEq_self`
+    apply ObsEq.coinductWith (fun 
+      (iTree.mk (State := State₁) curr₁ step₁) 
+      (iTree.mk (State := State₂) curr₂ step₂) =>
+      ∃ (H : State₂ = (Unit ⊕ (_ : A) × State₁)),
+      curr₂ = H.mpr (Sum.inr ⟨a, curr₁⟩) ∧
+      ∀ (s : State₁), 
+      step₂ (H ▸ (.inr ⟨a, s⟩)) = H.symm ▸ (step₁ s).mapState (.inr ⟨a, ·⟩)
+    )
+    case baseCase => 
+      simp [Obs.mapState]
+    case progress =>
+      rintro ⟨c₁, s₁⟩ ⟨c₂, s₂⟩ ⟨rfl, HC, Hs⟩
+      unfold ObsEq.func ObsRel.func unfold
+      cases _ : s₁ c₁ <;>
+      cases _ : s₂ c₂ <;>
+      simp [*, Obs.mapState]
+
+instance instEquiv {E R} : Equivalence (fun (x y : iTree E R) => x ≈ y) where
+  refl :=  ObsEq.refl
+  symm := ObsEq.symm _ _
+  trans := ObsEq.trans _ _ _
+
+instance instSetoid.{a,e,r} {E : Type a → Type e}{R : Type r}: Setoid (iTree.{a,e,r} E R) where
+  r := (· ≈ ·)
+  iseqv := instEquiv
+
+def iTree'.{a,e,r} (E : Type a → Type e) (R : Type r) : Type _ := Quotient (instSetoid (E := E) (R := R))
+
+set_option pp.universes true in #print iTree'
+
+def iTree'.mk {E : Type _ → Type _} {R : Type _}(it : iTree E R)  := Quotient.mk inferInstance it
+
+def iTree'.unfold (it' : iTree' E R) : Obs E R (iTree' E R) := 
+  it'.lift (fun it =>
+    match it.unfold with 
+    | Obs.ret v => Obs.ret v
+    | Obs.tau it₂ => Obs.tau (iTree'.mk it₂)
+    | Obs.vis ev k => 
+      Obs.vis ev (fun a => iTree'.mk (k a))
+  ) (by 
+    intros it₁ it₂ heq
+    match h₁ : it₁.unfold, h₂ : it₂.unfold with
+    | Obs.ret _, Obs.ret _ => 
+      simp [h₁, h₂]
+      grind only [ObsEq.unfold_eq_ret]
+    | Obs.vis (A := A₁) ev₁ k₁, Obs.vis (A := A₂) ev₂ k₂ =>
+      simp [*]
+      obtain ⟨rfl, rfl, ih⟩:= ObsEq.unfold_eq_vis h₁ h₂ heq
+      simp only [heq_eq_eq, true_and]
+      ext 
+      apply Quotient.sound
+      apply ih
+    | Obs.tau it₁', Obs.tau it₃' =>
+      simp [*]
+      apply Quotient.sound
+      apply ObsEq.unfold_eq_tau h₁ h₂ heq
+      /- grind [ObsEq.unfold_eq_tau] -/
+    | .ret .., .tau ..
+    | .ret .., .vis ..
+    | .vis .., .ret ..
+    | .vis .., .tau ..
+    | .tau .., .vis ..
+    | .tau .., .ret .. => 
+      grind)
+
+def iTree'.out (it' : iTree' E R) : iTree E R where
+    curr := it'
+    step := iTree'.unfold
+    
+def iTree'.ret {R : Type _} (v : R){E : Type _ → Type _} := iTree'.mk (.ret v : iTree E R)
+
+def iTree'.tau {R : Type _} {E : Type _ → Type _} (it : iTree' E R) := 
+    it.lift (Quotient.mk inferInstance <| iTree.tau ·) (by 
+      intros it it' heq; simp; apply Quotient.sound
+      apply ObsEq.tau_congr heq
+    )
+
+def iTree'.vis {A : Type a} {R : Type _}{E : Type a → Type _} (ev : E A) (k' : A → iTree' E R) : iTree' E R := 
+  let k := fun a => (k' a).out
+  iTree'.mk (.vis ev k)
+
+set_option pp.universes true in #print iTree'
+
+def iTree'.cases.{r,a,e,s} {R : Type r}{E : Type a → Type e} {motive : iTree'.{a,e,r,s} E R → Type _} 
+  (ret : (v : R) → motive (.ret v))
+  (vis : ∀ {A : Type a} (ev : E A) (k : A → iTree' E R), motive (iTree'.vis ev k))
+  (tau : (it : iTree' E R) → motive (.tau it)) : 
+    ∀ (it' : iTree' E R), motive it' := by
+  sorry
+
+end ThirdTry
+
+export SecondTry (eq wb wb.ret wb.vis wb.tauL wb.tauR wb.sync)
+
+end EqualitiesOverITrees
+
+@[simp, grind]
+instance : HasEquiv (iTree E R) where Equiv := SecondTry.eq
+
+-- This definition doesn't satisfy the monad laws up to equality, but it does
+-- follow then up to tau equality.
+
+/- theorem bindLeft_ret : it.unfold = .ret v → bindLeft f it = sorry := by -/
+/-   intros h -/
+/-   unfold bindLeft -/
+/-   sorry -/
+  
+
+theorem id_map {α : Type} (it : iTree E α) : bindLeft pure it ≈ it := by 
+  dsimp [HasEquiv.Equiv]
+  unfold eq
+  match h : it.unfold with 
+  | .ret v₁ => 
+    cases h₂ : it.step it.curr <;> (try simp [h₂, unfold] at h; done)
+    apply wb.tauL ?_ ?unfold ?next
+    case unfold =>
+      simp [unfold, bindLeft, h₂, Obs.bindVal, Obs.mapState]
+      rfl
+    apply wb.ret v₁ _ h
+    simp [unfold, pure, ret]
+    simp [unfold, h₂] at h
+    assumption
+  | .vis ev₁ k₁ => 
+    cases h₂ : it.step it.curr <;> (try simp [h₂, unfold] at h; done)
+    case vis A ev₁ k₁ =>
+    /- have := h -/
+    simp [h₂, unfold] at h
+    have ⟨rfl, h⟩ := h
+    simp at h
+    have ⟨h, h'⟩:= h
+    subst h h'
+    simp [bindLeft,  Obs.bindVal, Obs.mapState]
+    apply wb.vis ev₁ _ ev₁ _ ?left ?right
+    case left =>
+      simp [unfold, h₂, pure, ret]
+      sorry
+    all_goals sorry
+  | .tau it₁ => 
+    sorry
+
+instance  : LawfulMonad (iTree E) := .mk'
+   (id_map     := by 
+      simp only [Functor.map, bind, Pure.pure, Function.comp_id]
+      intros α it
+      have {State, curr, step} := it
+      simp [bindLeft, *]
+      sorry
+      /- induction it <;> simp [bindLeft, *] -/ 
+    )
+   (pure_bind  := by intros α β it f; simp only [bind, bindLeft])
+   (bind_assoc := by intros α β γ it f g; simp only [bind]; induction it <;> simp [bindLeft, *])
 
 end iTree
 
